Assoc.v
@@ -1,0 +1,59 @@
+Require Import List.
+
+Section Assoc.
+  
+  Context {A B:Type}.
+  Context (dec:forall a a':A, {a=a'} + {a<>a'}).
+  (* define lookup for assocation lists *)
+  Fixpoint lookup l a : option B
+    := match l with 
+       | nil => None
+       | (f',v')::os => if dec a f' then Some v' else lookup os a
+       end.
+  
+  Definition domain (l:list (A*B)) := map (@fst A B) l.
+  Definition codomain (l:list (A*B)) := map (@snd A B) l.
+
+  Lemma in_dom : forall {l} {a b}, In (a,b) l -> In a (domain l).
+    Proof.
+      unfold domain; induction l; simpl; trivial.
+      intros. destruct a; simpl in *; intuition.
+      inversion H0; intuition.
+      eauto.
+    Qed.
+
+  Lemma lookup_in : forall l {a:A} {b:B}, lookup l a = Some b -> In (a,b) l.
+  Proof.
+    induction l; simpl; intuition.
+    - discriminate.
+    - destruct (dec a a0).
+      + inversion H; intuition congruence.
+      + intuition.
+  Qed.
+
+  Lemma lookup_in_domain : forall l {a:A} {b:B}, lookup l a = Some b -> In a (domain l).
+  Proof.
+    induction l; simpl; intuition.
+    - discriminate.
+    - destruct (dec a a0); simpl.
+      + inversion H; intuition congruence.
+      + right; apply (IHl a b0); assumption.
+  Qed.
+
+  Lemma in_dom_lookup :  forall {l} {a:A}, In a (domain l) -> {v | lookup l a = Some v}.
+    Proof.
+      induction l; simpl; [tauto|]; intros.
+      destruct a; simpl in *.
+      destruct (dec a0 a); [eauto|].
+      apply IHl.
+      intuition congruence.
+    Qed.
+
+
+  Lemma in_lookup :  forall {l} {a:A} {b0:B}, In (a,b0) l -> {v | lookup l a = Some v}.
+  Proof.
+    Hint Resolve in_dom_lookup in_dom.
+    intros. eauto.
+  Qed.
+
+End Assoc.
